\documentclass[11pt]{article}

\usepackage{amsmath,amsfonts,amssymb,amsthm}
\usepackage{enumitem} 
\usepackage{mathtools}
\usepackage{MnSymbol}
\usepackage{calligra}
\usepackage[top=2cm,bottom=2cm,left=2cm,right=2cm,marginparwidth=1.75cm]{geometry}
\setlength{\parindent}{0cm}

\newcommand{\N}{\mathbb{N}}
\newcommand{\R}{\mathbb{R}}
\newcommand{\Z}{\mathbb{Z}}
\newcommand{\n}{\vspace{0.5cm}}

\pagenumbering{gobble}

\begin{document}
\title{\vspace{-1.5cm}MATH 4152 Homework 6}
  \author{Fletcher Gornick}
  \maketitle
  \begin{enumerate}
    \item Write down the associative and commutative laws for \(\vee\) and \(\leftrightarrow\).
      \begin{enumerate}
        \item[(\(\vee\))] given wffs \(\alpha, \beta, \gamma\) and truth evaluating function \(\bar\nu\), the following property holds:
          \[\bar\nu(((\alpha \vee \beta) \vee \gamma)) = \bar\nu((\alpha \vee (\beta \vee \gamma))) \]

        \item[(\(\leftrightarrow\))] given wffs \(\alpha, \beta, \gamma\) and truth evaluating function \(\bar\nu\), the following property holds:
          \[\bar\nu(((\alpha \leftrightarrow \beta) \leftrightarrow \gamma)) = \bar\nu((\alpha \leftrightarrow (\beta \leftrightarrow \gamma))) \]
      \end{enumerate} \n

    \item Write down the tautological equivalences corresponding to associative and commutative laws for \(\vee\) and \(\leftrightarrow\). (I.e. use 4(b).)
      \begin{itemize}
        \item Commutative - For wffs \(\alpha, \beta\):
          \[(\alpha \vee \beta) \models \leftmodels (\beta \vee \alpha) \quad\quad (\alpha \leftrightarrow \beta) \models \leftmodels (\beta \leftrightarrow \alpha)\]
          which can also be rewritten as:
          \[\models (\alpha \vee \beta) \leftrightarrow (\beta \vee \alpha) \quad \quad \models (\alpha \leftrightarrow \beta) \leftrightarrow (\beta \leftrightarrow \alpha)\]
        \item Associative - For wffs \(\alpha, \beta, \gamma\):
          \[((\alpha \vee \beta) \vee \gamma) \models \leftmodels (\alpha \vee (\beta \vee \gamma)) \quad\quad ((\alpha \leftrightarrow \beta) \leftrightarrow \gamma) \models \leftmodels (\alpha \leftrightarrow (\beta \leftrightarrow \gamma))\]
          which can also be rewritten as:
          \[\models ((\alpha \vee \beta) \vee \gamma) \leftrightarrow (\alpha \vee (\beta \vee \gamma)) \quad \quad \models ((\alpha \leftrightarrow \beta) \leftrightarrow \gamma) \leftrightarrow (\alpha \leftrightarrow (\beta \leftrightarrow \gamma))\]
      \end{itemize} \n

    \item For each of the four tautological equivalences in 2, write down the two corresponding tautological implications and their associated tautologies (obtained by using the simplist case of 4(a)).
      \begin{itemize}
        \item \((\alpha \vee \beta) \models \leftmodels (\beta \vee \alpha)\)
          \begin{enumerate}
            \item[(\(\models\))] \((\alpha \vee \beta) \models (\beta \vee \alpha)\)\\ associated tautology: \(\models ((\alpha \vee \beta) \to (\beta \vee \alpha))\)
            \item[(\(\leftmodels\))] \((\beta \vee \alpha) \models (\alpha \vee \beta)\)\\ associated tautology: \(\models ((\beta \vee \alpha) \to (\alpha \vee \beta))\)
          \end{enumerate} \n

        \item \((\alpha \leftrightarrow \beta) \models \leftmodels (\beta \leftrightarrow \alpha)\)
          \begin{enumerate}
            \item[(\(\models\))] \((\alpha \leftrightarrow \beta) \models (\beta \leftrightarrow \alpha)\)\\ associated tautology: \(\models ((\alpha \leftrightarrow \beta) \to (\beta \leftrightarrow \alpha))\)
            \item[(\(\leftmodels\))] \((\beta \leftrightarrow \alpha) \models (\alpha \leftrightarrow \beta)\)\\ associated tautology: \(\models ((\beta \leftrightarrow \alpha) \to (\alpha \leftrightarrow \beta))\)
          \end{enumerate} \n

        \item \(((\alpha \vee \beta) \vee \gamma) \models \leftmodels (\alpha \vee (\beta \vee \gamma))\)
          \begin{enumerate}
            \item[(\(\models\))] \(((\alpha \vee \beta) \vee \gamma) \models (\alpha \vee (\beta \vee \gamma))\)\\ associated tautology: \(\models (((\alpha \vee \beta) \vee \gamma) \to (\alpha \vee (\beta \vee \gamma)))\)
            \item[(\(\leftmodels\))] \((\alpha \vee (\beta \vee \gamma)) \models ((\alpha \vee \beta) \vee \gamma)\)\\ associated tautology: \(\models ((\alpha \vee (\beta \vee \gamma)) \to ((\alpha \vee \beta) \vee \gamma))\)
          \end{enumerate} \n

        \item \(((\alpha \leftrightarrow \beta) \leftrightarrow \gamma) \models \leftmodels (\alpha \leftrightarrow (\beta \leftrightarrow \gamma))\)
          \begin{enumerate}
            \item[(\(\models\))] \(((\alpha \leftrightarrow \beta) \leftrightarrow \gamma) \models (\alpha \leftrightarrow (\beta \leftrightarrow \gamma))\)\\ associated tautology: \(\models (((\alpha \leftrightarrow \beta) \leftrightarrow \gamma) \to (\alpha \leftrightarrow (\beta \leftrightarrow \gamma)))\)
            \item[(\(\leftmodels\))] \((\alpha \leftrightarrow (\beta \leftrightarrow \gamma)) \models ((\alpha \leftrightarrow \beta) \leftrightarrow \gamma)\)\\ associated tautology: \(\models ((\alpha \leftrightarrow (\beta \leftrightarrow \gamma)) \to ((\alpha \leftrightarrow \beta) \leftrightarrow \gamma))\)
          \end{enumerate}
      \end{itemize} \n

    \item Write down the tautological equivalences corresponding to the two De Morgan's laws.
      for wffs \(\alpha, \beta\):
      \[(\neg (\alpha \wedge \beta)) \models \leftmodels ((\neg \alpha) \vee (\neg \beta)) \quad \quad (\neg (\alpha \vee \beta)) \models \leftmodels ((\neg \alpha) \wedge (\neg \beta))\]

    \item For each of the two tautological equivalences in 4, write down the two corresponding tautological implications and their associated tautologies (obtained by using the simplist case of 4(a)).

    \item Using the exportation, i.e. not using the truth tables and truth values, prove:
      \begin{enumerate}
        \item \(((A \wedge B) \to C), \; A,B \vDash C\)
        \item \(((A \to B) \to C), \; (A \wedge B) \vDash C\)
      \end{enumerate}
  \end{enumerate}
\end{document}

